\documentstyle[a4]{article}

\begin{document}
\begin{description}
\item[apn2]$f^{s(n)}(x)=f \: of \: f^n(x)$
\item[appn2]$f^{s(n)}(x)=f^n(f(x))$
\item[sapn2]$s^{s(n)}(x)=s(s^n(x))$
\item[apn2thm]$f^{s(n)}(x)=f^n(f \: of \: x)$
\item[appn2thm]$f^{s(n)}(x)=f^n(f \: of \: x)$
\item[comapplem1]$::(h) \: of \: l_1 <> l_2 = h::(l_1 <> l_2)$
\item[comapplem2]$length(::(h) \: of \: l)=s(length(l))$
\item[conslem1]$::(f)^n(h::v_1)=::(f)^{s(n)}(v_1)$
\item[conslem2]$length(::(v)^n(h::t))=s(length(::(v)^n(t)))$
\item[hitlem1]$map(f)^n(map(f, v_1))=map(f)^{s(n)}(v_1)$
\item[hitlem2]$\lambda v_2. v_0 \: of \: v_2^{s(v_3)}(v_1)= v_0 \: of
\: \lambda v_2. v_0 \: of \: v_2^{v_3}(v_1)$
\item[nat1lem1]$s \: of \: s^n(a)=s^{s(n)}(a)$
\item[nat1lem2]$+(s(0))^n(a)+s(0)=+(s(0))^{s(n)}(a)$
\item[sapn2thm]$s^n(s(x))=s(s^n(x))$
\item[sapn2thm2]$s^{s(n)}(x)=s \: of \: s^n(x)$
\end{description}
\end{document}

